src/3d/Options.fsti
@@ -67,3 +67,5 @@ val get_emit_smt_encoding: unit -> ML bool
 val get_z3_test: unit -> ML (option string)
 
 val get_z3_witnesses: unit -> ML int
+
+val get_debug: unit -> ML bool
